TEOREMA PROVADO! + Funções totais relatório

dfa.v
@@ -5,44 +5,77 @@ Set Implicit Arguments.
 Unset Strict Implicit.
 Unset Printing Implicit Defensive.
 
+Inductive states {Q : Type} : Type :=
+  | sink_state
+  | state (q : Q).
+
 Record dfa (Q E : Type) := {
-  delta : Q -> E -> Q;
+  delta : Q -> E -> @states Q;
   initial_state : Q;
-  is_final : Q -> bool;
-  sink_state : Q
+  is_final : Q -> bool
 }.
 
-(* Extended delta:*)
+(* Extended transition function: *)
 
-Fixpoint delta' {Q E : Type} (g : dfa Q E) (q : Q) (w : list E) : Q :=
-  match w with
-  | [] => q
-  | e::w' => delta' g (g.(delta) q e) w'
+Fixpoint extended_delta {Q E : Type} (g : dfa Q E) (q : @states Q) (w : list E) : @states Q :=
+  match q with
+  | sink_state => sink_state
+  | state q' => match w with
+                | [] => state q'
+                | e::w' => extended_delta g (g.(delta) q' e) w'
+                end
   end.
+
+Theorem dist_extended_delta:
+  forall (Q E : Type) (g : dfa Q E) w w' q,
+    extended_delta g q (w ++ w') =
+    extended_delta g (extended_delta g q w) w'.
+Proof.
+  intros.
+  generalize dependent q.
+  generalize dependent w'.
+  induction w.
+  - intros. simpl. destruct q. reflexivity. reflexivity.
+  - intros. simpl. destruct q.
+    + destruct w'. reflexivity. reflexivity.
+    + rewrite IHw. reflexivity.
+Qed.
 
 (* Generated language: *)
 
 Definition in_language {Q E : Type} (g : dfa Q E) (w : list E) : Prop :=
-  ~ delta' g g.(initial_state) w = g.(sink_state).
+  ~ extended_delta g (state g.(initial_state)) w = sink_state.
 
-(* Example:
+Notation " x ==> g " := (in_language g x) (at level 60). (* ? *)
+
+Theorem prefix_closed:
+  forall (Q E : Type) (g : dfa Q E) w w',
+    (w ++ w') ==> g -> w ==> g.
+Proof.
+  unfold in_language, not.
+  intros.
+  rewrite dist_extended_delta in H. rewrite H0 in H. apply H.
+  destruct w'. reflexivity. reflexivity.
+Qed.
+
+(*
+Example:
 
 Inductive states1 : Type :=
   | q0 (* initial state *)
   | q1
-  | q2 (* final state *)
-  | q3.
+  | q2 (* final state *).
 
 Inductive events1 : Type :=
   | a
   | b.
 
-Definition delta1 (q:states1) (e:events1) : states1 :=
+Definition delta1 (q:states1) (e:events1) : @states states1 :=
   match q, e with
-  | q0, a => q1
-  | q1, b => q2
-  | q2, a => q1
-  | _, _ => q3
+  | q0, a => state q1
+  | q1, b => state q2
+  | q2, a => state q1
+  | _, _ => sink_state
   end.
 
 Definition is_final1 (q:states1) : bool :=
@@ -52,23 +85,24 @@ Definition is_final1 (q:states1) : bool :=
   end.
 
 Definition dfa1 :=
-  {| delta := delta1; initial_state := q0; is_final := is_final1; sink_state := q3 |}.
+  {| delta := delta1; initial_state := q0; is_final := is_final1 |}.
 
 Check dfa1.
 
-Compute delta' dfa1 q0 [a;b;a;b;a;b].
+Compute extended_delta dfa1 (state q0) [a;b;a;b;a;b].
 
-Theorem dfa1_test1 : in_language dfa1 [a;b;a;b;a;b].
+Theorem dfa1_test1 : [a;b;a;b;a;b] ==> dfa1.
 Proof.
-  unfold in_language, not.
+  unfold in_language.
+  unfold not.
   intros.
   discriminate H.
 Qed.
-
 *)
 
 Require Export Arith_base.
 Require Import BinPos BinInt BinNat Pnat Nnat.
+Require Import Omega.
 Local Open Scope Z_scope.
 
 Inductive events {E : Type} : Type :=
@@ -84,8 +118,149 @@ Fixpoint buffer_count {E : Type} (w : list (@events E)) : Z :=
   | _::w' => buffer_count w'
   end.
 
-Check [add;rem].
+Lemma buffer_add: forall (E : Type) (w : list (@events E)),
+  buffer_count (w ++ [add]) = buffer_count w + 1.
+Proof.
+  intros.
+  induction w.
+  - reflexivity.
+  - simpl. destruct a.
+    + rewrite IHw. reflexivity.
+    + rewrite IHw. omega.
+    + rewrite IHw. omega.
+Qed.
 
-(* not working *)
+Lemma buffer_rem: forall (E : Type) (w : list (@events E)),
+  buffer_count (w ++ [rem]) = buffer_count w - 1.
+Proof.
+  intros.
+  induction w.
+  - reflexivity.
+  - simpl. destruct a.
+    + rewrite IHw. omega.
+    + rewrite IHw. reflexivity.
+    + rewrite IHw. omega.
+Qed.
 
-Compute buffer_count [rem;add;add].
+Lemma buffer_other: forall (E : Type) (w : list (@events E)) (e : E),
+  buffer_count (w ++ [other e]) = buffer_count w.
+Proof.
+  intros.
+  induction w.
+  - reflexivity.
+  - simpl. destruct a.
+    + rewrite IHw. reflexivity.
+    + rewrite IHw. reflexivity.
+    + rewrite IHw. reflexivity.
+Qed.
+
+Lemma sla3: forall (Q E : Type) (g : dfa Q E) (q : Q) (e : E),
+  extended_delta g (state q) [e] = g.(delta) q e.
+Proof.
+  intros.
+  simpl.
+  destruct (delta g q e).
+  reflexivity.
+  reflexivity.
+Qed.
+
+Lemma th2:
+  forall (Q E : Type) (g : dfa Q (@events E)) (f : @states Q->Z),
+    (f(state g.(initial_state)) = 0 /\
+      forall (q : Q),
+        f(g.(delta) q add) >= f(state q) + 1 /\
+        f(g.(delta) q rem) >= f(state q) - 1 /\
+        (forall (e : E), f(g.(delta) q (other e)) >= f(state q))
+    ) -> (forall w, w ==> g -> buffer_count w <= f (extended_delta g (state g.(initial_state)) w)).
+Proof.
+  intros.
+  assert (forall q : Q, f (delta g q add) >= f (state q) + 1).
+  { apply H. }
+  assert (forall q : Q, f (delta g q rem) >= f (state q) - 1).
+  { apply H. }
+  assert (forall q : Q, (forall e : E, f (delta g q (other e)) >= f (state q))).
+  { apply H. }
+  destruct H.
+  induction w using @rev_ind.
+  - simpl. omega.
+  - simpl. destruct x.
+    + rewrite buffer_add.
+      assert (w ==> g).
+      { apply prefix_closed in H0. apply H0. }
+      apply IHw in H5.
+      assert (f (extended_delta g (state (initial_state g)) (w)) + 1 <= f (extended_delta g (state (initial_state g)) (w ++ [add]))).
+      { rewrite dist_extended_delta. remember (extended_delta g (state (initial_state g)) w). destruct s.
+        - apply prefix_closed in H0. unfold in_language in H0. unfold not in H0. symmetry in Heqs. apply H0 in Heqs.
+          destruct Heqs.
+        - rewrite sla3. assert (f (delta g q add) >= f (state q) + 1).
+          { apply H1. }
+          omega. }
+      omega.
+    + rewrite buffer_rem.
+      assert (w ==> g).
+      { apply prefix_closed in H0. apply H0. }
+      apply IHw in H5.
+      assert (f (extended_delta g (state (initial_state g)) (w)) - 1 <= f (extended_delta g (state (initial_state g)) (w ++ [rem]))).
+      { rewrite dist_extended_delta. remember (extended_delta g (state (initial_state g)) w). destruct s.
+        - apply prefix_closed in H0. unfold in_language in H0. unfold not in H0. symmetry in Heqs. apply H0 in Heqs.
+          destruct Heqs.
+        - rewrite sla3. assert (f (delta g q rem) >= f (state q) - 1).
+          { apply H2. }
+          omega. }
+      omega.
+    + rewrite buffer_other.
+      assert (w ==> g).
+      { apply prefix_closed in H0. apply H0. }
+      apply IHw in H5.
+      assert (f (extended_delta g (state (initial_state g)) (w)) <= f (extended_delta g (state (initial_state g)) (w ++ [other e]))).
+      { rewrite dist_extended_delta. remember (extended_delta g (state (initial_state g)) w). destruct s.
+        - apply prefix_closed in H0. unfold in_language in H0. unfold not in H0. symmetry in Heqs. apply H0 in Heqs.
+          destruct Heqs.
+        - rewrite sla3. assert (f (delta g q (other e)) >= f (state q)).
+          { apply H3. }
+          omega. }
+      omega.
+Qed.
+
+Theorem th1:
+  forall (Q E : Type) (g : dfa Q (@events E)) (n : Z),
+    (exists (f : @states Q->Z), f(state g.(initial_state)) = 0 /\
+      forall (q : Q),
+        f(state q) <= n /\
+        f(g.(delta) q add) >= f(state q) + 1 /\
+        f(g.(delta) q rem) >= f(state q) - 1 /\
+        (forall (e : E), f(g.(delta) q (other e)) >= f(state q))
+    ) -> (forall w, w ==> g -> buffer_count w <= n).
+Proof.
+  intros.
+  destruct H as [f [H1 H2]].
+  induction w using @rev_ind.
+  - assert (f (state (initial_state g)) <= n).
+    { apply H2. }
+    rewrite H1 in H.
+    simpl.
+    apply H.
+  - destruct x.
+    + assert (forall w, w ==> g -> buffer_count w <= f (extended_delta g (state g.(initial_state)) w)).
+      { apply th2. split.
+          apply H1. 
+          intros. split.
+          - apply H2.
+          - split.
+            + apply H2.
+            + apply H2. }
+      assert (buffer_count (w ++ [add]) <= f (extended_delta g (state (initial_state g)) (w ++ [add]))).
+      { apply H. apply H0. }
+      assert (f (extended_delta g (state (initial_state g)) (w ++ [add])) <= n).
+      { remember (extended_delta g (state (initial_state g)) (w ++ [add])).
+        destruct s.
+        - unfold in_language in H0. unfold not in H0. symmetry in Heqs. apply H0 in Heqs. destruct Heqs.
+        - apply H2. }
+      omega.
+    + apply prefix_closed in H0. apply IHw in H0.
+      rewrite buffer_rem.
+      omega.
+    + apply prefix_closed in H0. apply IHw in H0.
+      rewrite buffer_other. apply H0.
+Qed.
+
